coq/Conversion/ASN_Bitstring/Def.v
@@ -14,14 +14,14 @@ Section Atomic.
    *)
 
   (* [ 8.5.7.2 ] *)
-  Definition radix2bits (b : radix) : Z :=
+  Definition bits_of_radix (b : radix) : Z :=
     if Z.eqb b 2 then 0
     else if Z.eqb b 4 then 1
         else if Z.eqb b 8 then 2
               else if Z.eqb b 16 then 3
                   else 0.
 
-  Definition bits2radix (b : Z) : radix :=
+  Definition radix_of_bits (b : Z) : radix :=
     if Z.eqb b 0 then radix2
     else if Z.eqb b 1 then radix4
         else if Z.eqb b 2 then radix8
@@ -29,34 +29,34 @@ Section Atomic.
                   else radix2.
 
   (* [ 8.5.7.1 ] *)
-  Definition sign2bits (s : bool) : Z :=
+  Definition bits_of_sign (s : bool) : Z :=
     if s then 1 else 0.
 
-  Definition bits2sign (s : Z) : bool :=
+  Definition sign_of_bits (s : Z) : bool :=
     if (Z.eqb s 1) then true else false.
 
   (* [ 8.5.7.5 ] *)
-  Definition signif2bits (m : positive) : Z :=
+  Definition bits_of_signif (m : positive) : Z :=
     Zpos m.
 
-  Definition bits2signif (m : Z) : positive :=
+  Definition signif_of_bits (m : Z) : positive :=
     Z.to_pos m.
 
   (* [ 8.5.7.4 ] *)
-  Definition exp2bits (e_olen e : Z) : Z :=
+  Definition bits_of_exp (e_olen e : Z) : Z :=
     twos_comp_extended (8 * e_olen) e.
 
-  Definition bits2exp (e_olen e : Z) : Z :=
+  Definition exp_of_bits (e_olen e : Z) : Z :=
     twos_comp_extended (8 * e_olen) e.
 
 End Atomic.
 
-Definition finite_BER_to_bitstring
+Definition bitstring_of_finite_BER
             (s : bool) (b : radix) (f : Z) (m : positive) (e : Z) : option BER_bitstring :=
-  let m := signif2bits m in
-  let s := sign2bits s in
-  let bb := radix2bits b in
-  let e_olen := twos_olen e in let e := exp2bits e_olen e in
+  let m := bits_of_signif m in
+  let s := bits_of_sign s in
+  let bb := bits_of_radix b in
+  let e_olen := twos_olen e in let e := bits_of_exp e_olen e in
     if Z.ltb (e_olen) 4
     then
       match (valid_short_sumbool real_id_b (e_olen + olen m + 1) binary_bit s bb f (e_olen - 1) e m) with
@@ -69,15 +69,15 @@ Definition finite_BER_to_bitstring
           | left V => Some (long real_id_b (e_olen + olen m + 2) binary_bit s bb f 3 e_olen e m V)
       end.
 
-Definition BER_to_bitstring (f : BER_float) : option BER_bitstring :=
+Definition bitstring_of_BER (f : BER_float) : option BER_bitstring :=
   match f with
   | BER_zero s => Some (if s then special nzero_b else special pzero_b)
   | BER_infinity s => Some (if s then special ninf_b else special pinf_b)
   | BER_nan => Some (special nan_b)
-  | BER_finite s b ff m e _ => finite_BER_to_bitstring s b ff m e
+  | BER_finite s b ff m e _ => bitstring_of_finite_BER s b ff m e
   end.
 
-Definition bitstring_to_BER (b : BER_bitstring) : option BER_float :=
+Definition BER_of_bitstring (b : BER_bitstring) : option BER_float :=
   match b with
   | special val =>
     match classify_BER val with
@@ -89,19 +89,19 @@ Definition bitstring_to_BER (b : BER_bitstring) : option BER_float :=
     | None => None
     end
   | short id co t s bb ff ee e m _ =>
-    let s := (bits2sign s) in
-    let b := (bits2radix bb) in
-    let m := (bits2signif m) in
-    let e := (bits2exp (ee + 1) e) in
+    let s := (sign_of_bits s) in
+    let b := (radix_of_bits bb) in
+    let m := (signif_of_bits m) in
+    let e := (exp_of_bits (ee + 1) e) in
     match valid_BER_sumbool b ff m e with
     | right _ => None
     | left V => Some (BER_finite s b ff m e V)
     end
   | long id co t s bb ff ee eo e m _ =>
-    let s := (bits2sign s) in
-    let b := (bits2radix bb) in
-    let m := (bits2signif m) in
-    let e := (bits2exp (eo) e) in
+    let s := (sign_of_bits s) in
+    let b := (radix_of_bits bb) in
+    let m := (signif_of_bits m) in
+    let e := (exp_of_bits (eo) e) in
     match valid_BER_sumbool b ff m e with
     | right _ => None
     | left V => Some (BER_finite s b ff m e V)
