coq/Conversion/BinK.v
@@ -1,5 +1,5 @@
 Require Import ZArith.
-Require Import ASN1FP.Conversion.IEEE_ASN.Def.
+Require Import ASN1FP.Conversion.IEEE_ASN.DefProof.
 
 Open Scope Z.
 
@@ -18,11 +18,11 @@ Section B32.
   Let prec_lt_emax : prec < emax.
   Proof. subst prec. subst emax. reflexivity. Qed.
   
-  Definition b32_to_BER_abstract := IEEE_to_BER_exact prec emax.
+  Definition BER_of_b32_abstract := BER_of_IEEE_exact prec emax.
 
-  Definition BER_to_b32_abstract_exact := BER_to_IEEE_exact prec emax prec_gt_1.
+  Definition b32_of_BER_abstract_exact := IEEE_of_BER_exact prec emax prec_gt_1.
 
-  Definition BER_to_b32_abstract_rounded := BER_to_IEEE_rounded prec emax prec_gt_1 prec_lt_emax.
+  Definition b32_of_BER_abstract_rounded := IEEE_of_BER_rounded prec emax prec_gt_1 prec_lt_emax.
 
 End B32.
 
@@ -35,10 +35,10 @@ Section B64.
   Let prec_lt_emax : prec < emax.
   Proof. subst prec. subst emax. reflexivity. Qed.
   
-  Definition b64_to_BER_abstract := IEEE_to_BER_exact prec emax.
+  Definition BER_of_b64_abstract := BER_of_IEEE_exact prec emax.
 
-  Definition BER_to_b64_abstract_exact := BER_to_IEEE_exact prec emax prec_gt_1.
+  Definition b64_of_BER_abstract_exact := IEEE_of_BER_exact prec emax prec_gt_1.
 
-  Definition BER_to_b64_abstract_rounded := BER_to_IEEE_rounded prec emax prec_gt_1 prec_lt_emax.
+  Definition b64_of_BER_abstract_rounded := IEEE_of_BER_rounded prec emax prec_gt_1 prec_lt_emax.
 
 End B64.
