coq/Conversion/FullBin.v
@@ -1,7 +1,7 @@
 Require Import ZArith Basics.
 Require Import Aux.Option
         Types.ASNDef
-        Conversion.IEEE_ASN.Def
+        Conversion.IEEE_ASN.DefProof
         Conversion.ASN_Bitstring.Def
         Conversion.Bitstring_Bits.Def
         Conversion.BinK.
@@ -22,29 +22,29 @@ Notation "f >=> g" := (fun x => pbind (f x) g) (at level 50, left associativity)
 Section B32.
 
   Definition float32_to_BER_exact (target_radix : radix) (scaled : bool) : Z -> option Z :=
-      compose (b32_to_BER_abstract false) b32_of_bits >=> BER_to_bitstring >=>
-      compose ret bitstring_to_bits.
+      compose (BER_of_b32_abstract false) b32_of_bits >=> bitstring_of_BER >=>
+      compose ret bits_of_bitstring.
 
   Definition BER_to_float32_exact: Z -> option Z :=
-    bits_to_bitstring >=> bitstring_to_BER >=> BER_to_b32_abstract_exact >=>
+    bitstring_of_bits >=> BER_of_bitstring >=> b32_of_BER_abstract_exact >=>
              compose ret bits_of_b32.
 
   Definition BER_to_float32_rounded (rounding: mode): Z -> option Z :=
-    bits_to_bitstring >=> bitstring_to_BER >=> BER_to_b32_abstract_rounded rounding >=>
+    bitstring_of_bits >=> BER_of_bitstring >=> b32_of_BER_abstract_rounded rounding >=>
              compose ret bits_of_b32.
 End B32.
 
 Section B64.
 
   Definition float64_to_BER_exact (target_radix : radix) (scaled : bool) : Z -> option Z :=
-      compose (b64_to_BER_abstract false) b64_of_bits >=> BER_to_bitstring >=>
-      compose ret bitstring_to_bits.
+      compose (BER_of_b64_abstract false) b64_of_bits >=> bitstring_of_BER >=>
+      compose ret bits_of_bitstring.
 
   Definition BER_to_float64_exact: Z -> option Z :=
-    bits_to_bitstring >=> bitstring_to_BER >=> BER_to_b64_abstract_exact >=>
+    bitstring_of_bits >=> BER_of_bitstring >=> b64_of_BER_abstract_exact >=>
              compose ret bits_of_b64.
 
   Definition BER_to_float64_rounded (rounding: mode): Z -> option Z :=
-    bits_to_bitstring >=> bitstring_to_BER >=> BER_to_b64_abstract_rounded rounding >=>
+    bitstring_of_bits >=> BER_of_bitstring >=> b64_of_BER_abstract_rounded rounding >=>
              compose ret bits_of_b64.
 End B64.
